Sub.v done, skipped "variations"

Sub.v
@@ -1,6 +1,5 @@
 (** * Sub: Subtyping *)
 
-
 Require Export MoreStlc.
 
 (* ###################################################### *)
@@ -320,9 +319,39 @@ Require Export MoreStlc.
        f : Student -> Nat
        g : (Person -> Nat) -> Nat
     ... such that the application [g f] will get stuck during
-    execution.
+    execution. *)
+(*
+Student <: Person && Nat <: Nat
+==> (Student -> Nat) <: (Person -> Nat)
 
-[]
+(Student -> Nat) <: (Person -> Nat) && Nat <: Nat
+==> ((Person -> Nat) -> Nat) <: ((Student -> Nat) -> Nat)
+
+[g f] = [((Person -> Nat) -> Nat) (Student -> Nat)]
+==> [((Student -> Nat) -> Nat) (Student -> Nat)]
+==> [Nat]
+
+So, by above rule, [g f] should progress.
+let f := forall x : Student, x.gpa.
+let g := forall y : Person -> Nat, (y {James, 47}).
+
+[g f] ==>
+(f {James, 47})
+stuck!
+------------------------------------
+       f : Person -> C
+       g : (Student -> C) -> D
+
+Student <: Person
+(Person -> C) <: (Student -> C)
+[g f] = [((Student -> C) -> D) (Person -> C)]
+<: [((Student -> C) -> D) (Student -> C)]
+D!
+
+or,
+((Student -> C) -> D) <: ((Person -> C) -> D)
+[g f] <: [((Person -> C) -> D) (Person -> C)]
+D!
 *)
 
 (** *** Top *)
@@ -393,22 +422,47 @@ Require Export MoreStlc.
     and [U <: V].  Which of the following subtyping assertions
     are then true?  Write _true_ or _false_ after each one.  
     ([A], [B], and [C] here are base types.)
-
+*)
+(*
+-> can only appear with arrow rule.
     - [T->S <: T->S]
-
+true
     - [Top->U <: S->Top]
-
+true
     - [(C->C) -> (A*B)  <:  (C->C) -> (Top*B)]
-
+true
     - [T->T->U <: S->S->V]
-
+true
     - [(T->T)->U <: (S->S)->V]
-
+false
     - [((T->S)->T)->U <: ((S->T)->S)->V]
-
+<=> ((S->T)->S) <: ((T->S)->T)
+<=> T->S <: S->T
+<=> S <: T
+true
     - [S*V <: T*U]
-
+false
 []
+*)
+(*
+Assoc sound?
+-------------------------------------------
+T1 <: S1 && S2 <: T2
+(S1 -> S2) <: (T1 -> T2)
+
+(S1 -> S2) <: (T1 -> T2) && T3 <: S3
+((T1 -> T2) -> T3) <: ((S1 -> S2) -> S3)
+-------------------------------------------
+S2 <: T2 && T3 <: S3
+(T2 -> T3) <: (S2 -> S3)
+
+T1 <: S1 && (T2 -> T3) <: (S2 -> S3)
+(S1 -> (T2 -> T3)) <: (T1 -> (S2 -> S3))
+*)
+(*
+(T -> U) <: (S -> V)
+T -> (T -> U) <: S -> (S -> V)
+T -> (T -> (T -> U)) <: S -> (S -> (S -> V))
 *)
 
 (** **** Exercise: 2 stars (subtype_order) *)
@@ -421,10 +475,18 @@ Require Export MoreStlc.
 
 Write these types in order from the most specific to the most general.
 
+[Top -> Student] <:
+[Person -> Student] <:
+[Student -> Person] <:
+[Student -> Top] <:
+[Top]
 
 Where does the type [Top->Top->Student] fit into this order?
-
-
+[Top->Top->Student] <: [Top]
+[Top -> Student] <: [(Top->Top)->Student], but [Top->Top->Student] is not comparable
+[Person -> Student], [Top->Top->Student] : not comparable
+[Student -> Person], [Top->Top->Student] : not comparable
+[Student -> Top], [Top->Top->Student] : not comparable
 *)
 
 (** **** Exercise: 1 star (subtype_instances_tf_2) *)
@@ -433,57 +495,63 @@ Where does the type [Top->Top->Student] fit into this order?
       forall S T,
           S <: T  ->
           S->S   <:  T->T
+false
 
       forall S,
            S <: A->A ->
            exists T,
               S = T->T  /\  T <: A
+false
 
       forall S T1 T2,
            (S <: T1 -> T2) ->
            exists S1 S2,
               S = S1 -> S2  /\  T1 <: S1  /\  S2 <: T2 
+true
 
       exists S,
            S <: S->S 
+false
 
       exists S,
            S->S <: S   
+true, Top
 
       forall S T1 T2,
            S <: T1*T2 ->
            exists S1 S2,
-              S = S1*S2  /\  S1 <: T1  /\  S2 <: T2  
+              S = S1*S2  /\  S1 <: T1  /\  S2 <: T2
+true
 [] *)
 
 (** **** Exercise: 1 star (subtype_concepts_tf) *)
 (** Which of the following statements are true, and which are false?
     - There exists a type that is a supertype of every other type.
-
+true
     - There exists a type that is a subtype of every other type.
-
+false
     - There exists a pair type that is a supertype of every other
       pair type.
-
+true
     - There exists a pair type that is a subtype of every other
       pair type.
-
+false
     - There exists an arrow type that is a supertype of every other
       arrow type.
-
+false
     - There exists an arrow type that is a subtype of every other
       arrow type.
-
+false
     - There is an infinite descending chain of distinct types in the
       subtype relation---that is, an infinite sequence of types
       [S0], [S1], etc., such that all the [Si]'s are different and
       each [S(i+1)] is a subtype of [Si].
-
+true, adding a field inf...
     - There is an infinite _ascending_ chain of distinct types in
       the subtype relation---that is, an infinite sequence of types
       [S0], [S1], etc., such that all the [Si]'s are different and
       each [S(i+1)] is a supertype of [Si].
-
+false, there must be a Top.
 []
 *)
 
@@ -494,7 +562,10 @@ Where does the type [Top->Top->Student] fit into this order?
          ~(exists n, T = TBase n) ->
          exists S,
             S <: T  /\  S <> T
-]] 
+]]
+
+What is TBase?
+It seems right but not sure.
 []
 *)
 
@@ -508,6 +579,10 @@ Where does the type [Top->Top->Student] fit into this order?
 
    - What is the _largest_ type [T] that makes the same assertion true?
 
+\z:A.z \in A->A
+T <: A->A
+smallest : (Top->B) (if there exists, minimal elem s.t. B <: A)
+largest : (A->A)
 []
 *)
 
@@ -519,6 +594,10 @@ Where does the type [Top->Top->Student] fit into this order?
 
    - What is the _largest_ type [T] that makes the same assertion true?
 
+
+T : (A->A * B->B)
+smallest : (Top->(min A) * Top->(min B)) <: ~~ <: T
+largest : T <: ~~ <: (A->A * B->B)
 []
 *)
 
@@ -530,6 +609,16 @@ Where does the type [Top->Top->Student] fit into this order?
 
    - What is the _largest_ type [T] that makes the same assertion true?
 
+smallest :
+p:(A*T) <- (a, \z:A.z)
+A -> A <: T
+
+(T A) ==> A
+
+smallest
+A -> A
+largest
+Top -> (min A)
 []
 *)
 
@@ -546,6 +635,12 @@ Where does the type [Top->Top->Student] fit into this order?
    - What is the _largest_ type [T] that makes the same
      assertion true?
 
+(T A) ==> S
+
+T : Ta -> Tb
+s.t. A <: Ta && Tb <: S
+smallest : Top -> (min S)
+largest : A -> S
 []
 *)
 
@@ -554,7 +649,15 @@ Where does the type [Top->Top->Student] fit into this order?
     assertion true?
       exists S, exists t, 
         empty |- (\x:T. x x) t : S
-]] 
+]]
+
+
+(x x) : S
+x : xa -> xb
+x <: xa && xb <: S
+
+x := Top -> S
+otherwise, infinite chain?
 []
 *)
 
@@ -562,7 +665,10 @@ Where does the type [Top->Top->Student] fit into this order?
 (** What is the _smallest_ type [T] that makes the following
     assertion true?
       empty |- (\x:Top. x) ((\z:A.z) , (\z:B.z)) : T
-]] 
+]]
+
+(Top -> Top) (A->A * B->B) : T
+Top
 []
 *)
 
@@ -574,6 +680,22 @@ Where does the type [Top->Top->Student] fit into this order?
     [{x:A,y:B}] and [{y:B,x:A}] are different.)
 
 
+I considered A and C does not have any other subtype order except with Top.
+
+2-tuple (  *2! for permutation)
+A, C->Top
+A, Top
+Top, C->C
+Top, C->Top
+Top, Top
+
+1-tuple
+Top
+A
+C->C
+C->Top
+
+14?
 []
 *)
 
@@ -588,6 +710,8 @@ intuitively corresponds to the "depth" subtyping rule for records. Extending the
 for products.
 Is this a good idea? Briefly explain why or why not.
 
+
+It seems no problem, quite looks like matter of design..
 []
 *)
 
@@ -622,13 +746,18 @@ Inductive ty : Type :=
   | TBase  : id -> ty
   | TArrow : ty -> ty -> ty
   | TUnit  : ty
-.
+  | TProd  : ty -> ty -> ty
+  | TRNil : ty
+  | TRCons : id -> ty -> ty -> ty.
+
 
 Tactic Notation "T_cases" tactic(first) ident(c) :=
   first;
   [ Case_aux c "TTop" | Case_aux c "TBool" 
   | Case_aux c "TBase" | Case_aux c "TArrow" 
-  | Case_aux c "TUnit" | 
+  | Case_aux c "TUnit"
+  | Case_aux c "TProd"
+  | Case_aux c "TRNil" | Case_aux c "TRCons"             
   ].
 
 Inductive tm : Type :=
@@ -638,15 +767,26 @@ Inductive tm : Type :=
   | ttrue : tm
   | tfalse : tm
   | tif : tm -> tm -> tm -> tm
-  | tunit : tm 
-.
+  | tunit : tm
+
+  | tpair : tm -> tm -> tm
+  | tfst : tm -> tm
+  | tsnd : tm -> tm
+
+  | tproj : tm -> id -> tm
+  | trnil :  tm
+  | trcons : id -> tm -> tm -> tm.
 
 Tactic Notation "t_cases" tactic(first) ident(c) :=
   first;
   [ Case_aux c "tvar" | Case_aux c "tapp" 
   | Case_aux c "tabs" | Case_aux c "ttrue" 
   | Case_aux c "tfalse" | Case_aux c "tif"
-  | Case_aux c "tunit" 
+  | Case_aux c "tunit"
+  | Case_aux c "tpair"
+  | Case_aux c "tfst"
+  | Case_aux c "tsnd"
+  | Case_aux c "tproj" | Case_aux c "trnil" | Case_aux c "trcons"             
   ].
 
 (* ################################### *)
@@ -654,6 +794,46 @@ Tactic Notation "t_cases" tactic(first) ident(c) :=
 
 (** The definition of substitution remains exactly the same as for the
     pure STLC. *)
+
+Inductive record_ty : ty -> Prop :=
+  | RTnil : 
+        record_ty TRNil
+  | RTcons : forall i T1 T2,
+        record_ty (TRCons i T1 T2).
+
+Inductive record_tm : tm -> Prop :=
+  | rtnil :
+        record_tm trnil
+  | rtcons : forall i t1 t2,
+        record_tm (trcons i t1 t2).
+
+Inductive well_formed_ty : ty -> Prop :=
+  | wfTBase : forall i,
+        well_formed_ty (TBase i)
+  | wfTArrow : forall T1 T2,
+        well_formed_ty T1 ->
+        well_formed_ty T2 ->
+        well_formed_ty (TArrow T1 T2)
+  | wfTRNil :
+        well_formed_ty TRNil
+  | wfTRCons : forall i T1 T2,
+        well_formed_ty T1 ->
+        well_formed_ty T2 ->
+        record_ty T2 ->
+        well_formed_ty (TRCons i T1 T2)
+  | wfTProd : forall T1 T2,
+        well_formed_ty T1 ->
+        well_formed_ty T2 ->
+        well_formed_ty (TProd T1 T2)
+  | wfTTop :
+        well_formed_ty TTop
+  | wfTUnit :
+        well_formed_ty TUnit
+  | wfTBool :
+        well_formed_ty TBool
+.
+
+Hint Constructors record_ty record_tm well_formed_ty.
 
 Fixpoint subst (x:id) (s:tm)  (t:tm) : tm :=
   match t with
@@ -670,7 +850,18 @@ Fixpoint subst (x:id) (s:tm)  (t:tm) : tm :=
   | tif t1 t2 t3 => 
       tif (subst x s t1) (subst x s t2) (subst x s t3)
   | tunit => 
-      tunit 
+      tunit
+
+  | tpair t1 t2 => 
+      tpair (subst x s t1) (subst x s t2)
+  | tfst t1 => 
+      tfst (subst x s t1)
+  | tsnd t1 => 
+      tsnd (subst x s t1)
+
+  | tproj t1 i => tproj (subst x s t1) i
+  | trnil => trnil
+  | trcons i t1 tr1 => trcons i (subst x s t1) (subst x s tr1)
   end.
 
 Notation "'[' x ':=' s ']' t" := (subst x s t) (at level 20).
@@ -690,9 +881,35 @@ Inductive value : tm -> Prop :=
       value tfalse
   | v_unit : 
       value tunit
+
+  | v_rnil : value trnil
+  | v_rcons : forall i v1 vr,
+      value v1 ->
+      value vr ->
+      value (trcons i v1 vr)
+
+  | v_pair : forall v1 v2,
+      value v1 ->
+      value v2 ->
+      value (tpair v1 v2)
 .
 
+
 Hint Constructors value.
+
+
+Fixpoint Tlookup (i:id) (Tr:ty) : option ty :=
+  match Tr with
+  | TRCons i' T Tr' => if eq_id_dec i i' then Some T else Tlookup i Tr'
+  | _ => None
+  end.
+
+Fixpoint tlookup (i:id) (tr:tm) : option tm :=
+  match tr with
+  | trcons i' t tr' => if eq_id_dec i i' then Some t else tlookup i tr'
+  | _ => None
+  end.
+
 
 Reserved Notation "t1 '==>' t2" (at level 40).
 
@@ -714,16 +931,280 @@ Inductive step : tm -> tm -> Prop :=
   | ST_If : forall t1 t1' t2 t3,
       t1 ==> t1' ->
       (tif t1 t2 t3) ==> (tif t1' t2 t3)
+                     
+  | ST_Pair1 : forall t1 t1' t2,
+        t1 ==> t1' ->
+        (tpair t1 t2) ==> (tpair t1' t2)
+  | ST_Pair2 : forall v1 t2 t2',
+        value v1 ->
+        t2 ==> t2' ->
+        (tpair v1 t2) ==> (tpair v1 t2')
+  | ST_Fst1 : forall t1 t1',
+        t1 ==> t1' ->
+        (tfst t1) ==> (tfst t1')
+  | ST_FstPair : forall v1 v2,
+        value v1 ->
+        value v2 ->
+        (tfst (tpair v1 v2)) ==> v1
+  | ST_Snd1 : forall t1 t1',
+        t1 ==> t1' ->
+        (tsnd t1) ==> (tsnd t1')
+  | ST_SndPair : forall v1 v2,
+        value v1 ->
+        value v2 ->
+        (tsnd (tpair v1 v2)) ==> v2
+
+
+  | ST_Proj1 : forall t1 t1' i,
+        t1 ==> t1' ->
+        (tproj t1 i) ==> (tproj t1' i)
+  | ST_ProjRcd : forall tr i vi,
+        value tr ->
+        tlookup i tr = Some vi ->
+        (tproj tr i) ==> vi
+  | ST_Rcd_Head : forall i t1 t1' tr2,
+        t1 ==> t1' ->
+        (trcons i t1 tr2) ==> (trcons i t1' tr2)
+  | ST_Rcd_Tail : forall i v1 tr2 tr2',
+        value v1 ->
+        tr2 ==> tr2' ->
+        (trcons i v1 tr2) ==> (trcons i v1 tr2')
+
 where "t1 '==>' t2" := (step t1 t2).
 
 Tactic Notation "step_cases" tactic(first) ident(c) :=
   first;
   [ Case_aux c "ST_AppAbs" | Case_aux c "ST_App1" 
   | Case_aux c "ST_App2" | Case_aux c "ST_IfTrue" 
-  | Case_aux c "ST_IfFalse" | Case_aux c "ST_If"  
+  | Case_aux c "ST_IfFalse" | Case_aux c "ST_If"
+  | Case_aux c "ST_Pair1"
+  | Case_aux c "ST_Pair2"
+  | Case_aux c "ST_Fst1"
+  | Case_aux c "ST_FstPair"
+  | Case_aux c "ST_Snd1"
+  | Case_aux c "ST_SndPair"
+  | Case_aux c "ST_Proj1" | Case_aux c "ST_ProjRcd"
+  | Case_aux c "ST_Rcd_Head" | Case_aux c "ST_Rcd_Tail"
   ].
 
 Hint Constructors step.
+
+
+(* from MoreStlc.v *)
+
+
+
+(* ###################################################################### *)
+(** ** Records *)
+
+(** As a final example of a basic extension of the STLC, let's
+    look briefly at how to define _records_ and their types.
+    Intuitively, records can be obtained from pairs by two kinds of
+    generalization: they are n-ary products (rather than just binary)
+    and their fields are accessed by _label_ (rather than position).
+
+    Conceptually, this extension is a straightforward generalization
+    of pairs and product types, but notationally it becomes a little
+    heavier; for this reason, we postpone its formal treatment to a
+    separate chapter ([Records]). *)
+
+(** Records are not included in the extended exercise below, but
+    they will be useful to motivate the [Sub] chapter. *)
+
+(** Syntax:
+<<
+       t ::=                          Terms
+           | ...
+           | {i1=t1, ..., in=tn}         record 
+           | t.i                         projection
+
+       v ::=                          Values
+           | ...
+           | {i1=v1, ..., in=vn}         record value
+
+       T ::=                          Types
+           | ...
+           | {i1:T1, ..., in:Tn}         record type
+>> 
+   Intuitively, the generalization is pretty obvious.  But it's worth
+   noticing that what we've actually written is rather informal: in
+   particular, we've written "[...]" in several places to mean "any
+   number of these," and we've omitted explicit mention of the usual
+   side-condition that the labels of a record should not contain
+   repetitions. *)
+(* It is possible to devise informal notations that are
+   more precise, but these tend to be quite heavy and to obscure the
+   main points of the definitions.  So we'll leave these a bit loose
+   here (they are informal anyway, after all) and do the work of
+   tightening things up elsewhere (in chapter [Records]). *)
+
+(**
+   Reduction:
+                              ti ==> ti'
+                 ------------------------------------                  (ST_Rcd)
+                     {i1=v1, ..., im=vm, in=ti, ...}
+                 ==> {i1=v1, ..., im=vm, in=ti', ...}
+
+                              t1 ==> t1'
+                            --------------                           (ST_Proj1)
+                            t1.i ==> t1'.i
+
+                      -------------------------                    (ST_ProjRcd)
+                      {..., i=vi, ...}.i ==> vi
+   Again, these rules are a bit informal.  For example, the first rule
+   is intended to be read "if [ti] is the leftmost field that is not a
+   value and if [ti] steps to [ti'], then the whole record steps..."
+   In the last rule, the intention is that there should only be one
+   field called i, and that all the other fields must contain values. *)
+
+(**
+   Typing:
+            Gamma |- t1 : T1     ...     Gamma |- tn : Tn
+          --------------------------------------------------            (T_Rcd)
+          Gamma |- {i1=t1, ..., in=tn} : {i1:T1, ..., in:Tn}
+
+                    Gamma |- t : {..., i:Ti, ...}
+                    -----------------------------                      (T_Proj)
+                          Gamma |- t.i : Ti
+
+*)
+
+(* ###################################################################### *)
+(** *** Encoding Records (Optional) *)
+
+(** There are several ways to make the above definitions precise.  
+
+      - We can directly formalize the syntactic forms and inference
+        rules, staying as close as possible to the form we've given
+        them above.  This is conceptually straightforward, and it's
+        probably what we'd want to do if we were building a real
+        compiler -- in particular, it will allow is to print error
+        messages in the form that programmers will find easy to
+        understand.  But the formal versions of the rules will not be
+        pretty at all!
+
+      - We could look for a smoother way of presenting records -- for
+        example, a binary presentation with one constructor for the
+        empty record and another constructor for adding a single field
+        to an existing record, instead of a single monolithic
+        constructor that builds a whole record at once.  This is the
+        right way to go if we are primarily interested in studying the
+        metatheory of the calculi with records, since it leads to
+        clean and elegant definitions and proofs.  Chapter [Records]
+        shows how this can be done.
+
+      - Alternatively, if we like, we can avoid formalizing records
+        altogether, by stipulating that record notations are just
+        informal shorthands for more complex expressions involving
+        pairs and product types.  We sketch this approach here.
+
+    First, observe that we can encode arbitrary-size tuples using
+    nested pairs and the [unit] value.  To avoid overloading the pair
+    notation [(t1,t2)], we'll use curly braces without labels to write
+    down tuples, so [{}] is the empty tuple, [{5}] is a singleton
+    tuple, [{5,6}] is a 2-tuple (morally the same as a pair),
+    [{5,6,7}] is a triple, etc.  
+<<
+    {}                 ---->  unit
+    {t1, t2, ..., tn}  ---->  (t1, trest)
+                              where {t2, ..., tn} ----> trest
+>>
+    Similarly, we can encode tuple types using nested product types:
+<<
+    {}                 ---->  Unit
+    {T1, T2, ..., Tn}  ---->  T1 * TRest
+                              where {T2, ..., Tn} ----> TRest
+>>
+    The operation of projecting a field from a tuple can be encoded
+    using a sequence of second projections followed by a first projection: 
+<<
+    t.0        ---->  t.fst
+    t.(n+1)    ---->  (t.snd).n
+>>
+
+    Next, suppose that there is some total ordering on record labels,
+    so that we can associate each label with a unique natural number.
+    This number is called the _position_ of the label.  For example,
+    we might assign positions like this:
+<<
+      LABEL   POSITION
+      a       0
+      b       1
+      c       2
+      ...     ...
+      foo     1004
+      ...     ...
+      bar     10562
+      ...     ...
+>>       
+
+    We use these positions to encode record values as tuples (i.e., as
+    nested pairs) by sorting the fields according to their positions.
+    For example:
+<<
+      {a=5, b=6}      ---->   {5,6}
+      {a=5, c=7}      ---->   {5,unit,7}
+      {c=7, a=5}      ---->   {5,unit,7}
+      {c=5, b=3}      ---->   {unit,3,5}
+      {f=8,c=5,a=7}   ---->   {7,unit,5,unit,unit,8}
+      {f=8,c=5}       ---->   {unit,unit,5,unit,unit,8}
+>>
+    Note that each field appears in the position associated with its
+    label, that the size of the tuple is determined by the label with
+    the highest position, and that we fill in unused positions with
+    [unit].  
+
+    We do exactly the same thing with record types:
+<<
+      {a:Nat, b:Nat}      ---->   {Nat,Nat}
+      {c:Nat, a:Nat}      ---->   {Nat,Unit,Nat}
+      {f:Nat,c:Nat}       ---->   {Unit,Unit,Nat,Unit,Unit,Nat}
+>>
+
+    Finally, record projection is encoded as a tuple projection from
+    the appropriate position:
+<<
+      t.l  ---->  t.(position of l)
+>>    
+
+    It is not hard to check that all the typing rules for the original
+    "direct" presentation of records are validated by this
+    encoding.  (The reduction rules are "almost validated" -- not
+    quite, because the encoding reorders fields.) *)
+
+(** Of course, this encoding will not be very efficient if we
+    happen to use a record with label [bar]!  But things are not
+    actually as bad as they might seem: for example, if we assume that
+    our compiler can see the whole program at the same time, we can
+    _choose_ the numbering of labels so that we assign small positions
+    to the most frequently used labels.  Indeed, there are industrial
+    compilers that essentially do this! *)
+
+(** *** Variants (Optional Reading) *)
+
+(** Just as products can be generalized to records, sums can be
+    generalized to n-ary labeled types called _variants_.  Instead of
+    [T1+T2], we can write something like [<l1:T1,l2:T2,...ln:Tn>]
+    where [l1],[l2],... are field labels which are used both to build
+    instances and as case arm labels.  
+
+    These n-ary variants give us almost enough mechanism to build
+    arbitrary inductive data types like lists and trees from
+    scratch -- the only thing missing is a way to allow _recursion_ in
+    type definitions.  We won't cover this here, but detailed
+    treatments can be found in many textbooks -- e.g., Types and
+    Programming Languages. *)
+
+
+
+
+
+
+
+
+
+
+
 
 (* ###################################################################### *)
 (** ** Subtyping *)
@@ -737,32 +1218,337 @@ Hint Constructors step.
 
 Reserved Notation "T '<:' U" (at level 40).
 
+(* well_formed_ty ??? *)
+
+Inductive is_sublist : ty -> ty -> Prop :=
+  | sub_nil : forall l,
+      is_sublist TRNil l
+  | sub_append : forall i Ti l1 l2,
+      is_sublist l1 l2 ->
+      Tlookup i l2 = Some Ti ->
+      is_sublist (TRCons i Ti l1) l2
+.
+(*
+  S <: T ->
+  Tlookup i T = Some T1 ->
+(*  Tlookup i S = Some T1. *)
+  exists T2, (Tlookup i S = Some T2) /\ (T2 <: T1).
+*)
+
+Hint Constructors is_sublist.
+
+Example is_sublist_ex0 :
+  (is_sublist TRNil TRNil).
+Proof. auto. Qed.
+
+Example is_sublist_ex1 :
+  (is_sublist TRNil (TRCons (Id 20) (TBase (Id 25)) TRNil)).
+Proof. auto. Qed.
+
+Example is_sublist_ex2 :
+  (is_sublist 
+     (TRCons (Id 30) (TBase (Id 35)) (TRCons (Id 20) (TBase (Id 25)) TRNil))
+     (TRCons (Id 20) (TBase (Id 25)) (TRCons (Id 30) (TBase (Id 35)) TRNil))
+  ).
+Proof. auto. Qed.
+
+
+(*
+Set Implicit Arguments.
+
+Local Notation "[ ]" := nil.
+(* Local Notation "[ a ; .. ; b ]" := (a :: .. (b :: []) ..). *)
+
+Section Permutation.
+
+Variable A:Type.
+
+Inductive Permutation : list A -> list A -> Prop :=
+| perm_nil: Permutation [] []
+| perm_skip x l l' : Permutation l l' -> Permutation (x::l) (x::l')
+| perm_swap x y l : Permutation (y::x::l) (x::y::l)
+| perm_trans l l' l'' : Permutation l l' -> Permutation l' l'' -> Permutation l l''.
+
+Local Hint Constructors Permutation.
+
+Theorem Permutation_nil : forall (l : list A), Permutation [] l -> l = nil.
+
+Theorem Permutation_nil_cons : forall (l : list A) (x : A), ~ Permutation nil (x::l).
+
+Permutation over lists is a equivalence relation
+
+Theorem Permutation_refl : forall l : list A, Permutation l l.
+
+Theorem Permutation_sym : forall l l' : list A, Permutation l l' -> Permutation l' l.
+
+Theorem Permutation_trans : forall l l' l'' : list A, Permutation l l' -> Permutation l' l'' -> Permutation l l''.
+
+End Permutation.
+
+Hint Resolve Permutation_refl perm_nil perm_skip.
+
+
+Local Hint Resolve perm_swap perm_trans.
+Local Hint Resolve Permutation_sym Permutation_trans.
+
+
+Instance Permutation_Equivalence A : Equivalence (@Permutation A) | 10 := {
+  Equivalence_Reflexive := @Permutation_refl A ;
+  Equivalence_Symmetric := @Permutation_sym A ;
+  Equivalence_Transitive := @Permutation_trans A }.
+
+Add Parametric Morphism A (a:A) : (cons a)
+  with signature @Permutation A ==> @Permutation A
+  as Permutation_cons.
+
+Section Permutation_properties.
+
+Variable A:Type.
+
+Implicit Types a b : A.
+Implicit Types l m : list A.
+
+Compatibility with others operations on lists
+
+Theorem Permutation_in : forall (l l' : list A) (x : A), Permutation l l' -> In x l -> In x l'.
+
+Lemma Permutation_app_tail : forall (l l' tl : list A), Permutation l l' -> Permutation (l++tl) (l'++tl).
+
+Lemma Permutation_app_head : forall (l tl tl' : list A), Permutation tl tl' -> Permutation (l++tl) (l++tl').
+
+Theorem Permutation_app : forall (l m l' m' : list A), Permutation l l' -> Permutation m m' -> Permutation (l++m) (l'++m').
+
+Add Parametric Morphism : (@app A)
+  with signature @Permutation A ==> @Permutation A ==> @Permutation A
+  as Permutation_app'.
+Qed.
+
+Lemma Permutation_add_inside : forall a (l l' tl tl' : list A),
+  Permutation l l' -> Permutation tl tl' ->
+  Permutation (l ++ a :: tl) (l' ++ a :: tl').
+
+Lemma Permutation_cons_append : forall (l : list A) x,
+  Permutation (x :: l) (l ++ x :: nil).
+Local Hint Resolve Permutation_cons_append.
+
+Theorem Permutation_app_comm : forall (l l' : list A),
+  Permutation (l ++ l') (l' ++ l).
+Local Hint Resolve Permutation_app_comm.
+
+Theorem Permutation_cons_app : forall (l l1 l2:list A) a,
+  Permutation l (l1 ++ l2) -> Permutation (a :: l) (l1 ++ a :: l2).
+Local Hint Resolve Permutation_cons_app.
+
+Theorem Permutation_middle : forall (l1 l2:list A) a,
+  Permutation (a :: l1 ++ l2) (l1 ++ a :: l2).
+Local Hint Resolve Permutation_middle.
+
+Theorem Permutation_rev : forall (l : list A), Permutation l (rev l).
+
+Add Parametric Morphism : (@rev A)
+  with signature @Permutation A ==> @Permutation A as Permutation_rev'.
+
+Theorem Permutation_length : forall (l l' : list A), Permutation l l' -> length l = length l'.
+
+Theorem Permutation_ind_bis :
+ forall P : list A -> list A -> Prop,
+   P [] [] ->
+   (forall x l l', Permutation l l' -> P l l' -> P (x :: l) (x :: l')) ->
+   (forall x y l l', Permutation l l' -> P l l' -> P (y :: x :: l) (x :: y :: l')) ->
+   (forall l l' l'', Permutation l l' -> P l l' -> Permutation l' l'' -> P l' l'' -> P l l'') ->
+   forall l l', Permutation l l' -> P l l'.
+
+Ltac break_list l x l' H :=
+  destruct l as [|x l']; simpl in *;
+  injection H; intros; subst; clear H.
+
+Theorem Permutation_nil_app_cons : forall (l l' : list A) (x : A), ~ Permutation nil (l++x::l').
+
+Theorem Permutation_app_inv : forall (l1 l2 l3 l4:list A) a,
+  Permutation (l1++a::l2) (l3++a::l4) -> Permutation (l1++l2) (l3 ++ l4).
+
+Theorem Permutation_cons_inv :
+   forall l l' a, Permutation (a::l) (a::l') -> Permutation l l'.
+
+Theorem Permutation_cons_app_inv :
+   forall l l1 l2 a, Permutation (a :: l) (l1 ++ a :: l2) -> Permutation l (l1 ++ l2).
+
+Theorem Permutation_app_inv_l :
+    forall l l1 l2, Permutation (l ++ l1) (l ++ l2) -> Permutation l1 l2.
+
+Theorem Permutation_app_inv_r :
+   forall l l1 l2, Permutation (l1 ++ l) (l2 ++ l) -> Permutation l1 l2.
+
+Lemma Permutation_length_1_inv: forall a l, Permutation [a] l -> l = [a].
+
+Lemma Permutation_length_1: forall a b, Permutation [a] [b] -> a = b.
+
+Lemma Permutation_length_2_inv :
+  forall a1 a2 l, Permutation [a1;a2] l -> l = [a1;a2] \/ l = [a2;a1].
+
+Lemma Permutation_length_2 :
+  forall a1 a2 b1 b2, Permutation [a1;a2] [b1;b2] ->
+    a1 = b1 /\ a2 = b2 \/ a1 = b2 /\ a2 = b1.
+
+Lemma NoDup_Permutation : forall l l',
+  NoDup l -> NoDup l' -> (forall x:A, In x l <-> In x l') -> Permutation l l'.
+
+End Permutation_properties.
+
+Section Permutation_map.
+
+Variable A B : Type.
+Variable f : A -> B.
+
+Add Parametric Morphism : (map f)
+  with signature (@Permutation A) ==> (@Permutation B) as Permutation_map_aux.
+
+Lemma Permutation_map :
+  forall l l', Permutation l l' -> Permutation (map f l) (map f l').
+
+End Permutation_map.
+*)
+
 Inductive subtype : ty -> ty -> Prop :=
   | S_Refl : forall T,
+      well_formed_ty T ->
       T <: T
   | S_Trans : forall S U T,
       S <: U ->
       U <: T ->
       S <: T
   | S_Top : forall S,
+      well_formed_ty S ->
       S <: TTop
   | S_Arrow : forall S1 S2 T1 T2,
       T1 <: S1 ->
       S2 <: T2 ->
       (TArrow S1 S2) <: (TArrow T1 T2)
+
+  | S_Prod : forall S1 S2 T1 T2,
+      S1 <: T1 ->
+      S2 <: T2 ->
+      (TProd S1 S2) <: (TProd T1 T2)
+
+  | S_RcdWidthBoth : forall i Ti T1 T2,
+      well_formed_ty Ti ->
+      record_ty T1 ->
+      record_ty T2 ->
+      T1 <: T2 ->
+      TRCons i Ti T1 <: TRCons i Ti T2
+  | S_RcdWidthNil : forall T,
+      well_formed_ty T ->
+      record_ty T ->
+      T <: TRNil
+                               (*
+  | S_RcdWidthSub : forall i Ti T1 T2,
+      record_ty T1 ->
+      record_ty T2 ->
+      T1 <: T2 ->
+      TRCons i Ti T1 <: T2
+*)
+  | S_RcdDepth : forall i T1 T2 T,
+      well_formed_ty T ->
+      record_ty T ->
+      T1 <: T2 ->
+      TRCons i T1 T <: TRCons i T2 T
+
+  | S_RcdPerm : forall T1 T2,
+      well_formed_ty T1 ->
+      well_formed_ty T2 ->
+      record_ty T1 ->
+      record_ty T2 ->
+      is_sublist T1 T2 -> is_sublist T2 T1 ->
+      T1 <: T2
+                         (*
+  | S_ProdWidth1 : forall S1 S2,
+      (TProd S1 S2) <: S1
+  | S_ProdWidth2 : forall S1 S2,
+      (TProd S1 S2) <: S2
+*)
+(*
+  | S_ProdPerm : forall S1 S2,
+      (TProd S1 S2) <: (TProd S2 S1)
+*)
+                         (*
+  | S_RcdWidth : 
+  | S_RcdDepth : 
+  | S_RcdPerm :
+*)
+
 where "T '<:' U" := (subtype T U).
+
+
+(*
+
+                        for each jk in j1..jn,
+                    exists ip in i1..im, such that
+                          jk=ip and Sp <: Tk
+                  ----------------------------------                    (S_Rcd)
+                  {i1:S1...im:Sm} <: {j1:T1...jn:Tn}
+
+
+                               n > m
+                 ---------------------------------                 (S_RcdWidth)
+                 {i1:T1...in:Tn} <: {i1:T1...im:Tm} 
+
+                       S1 <: T1  ...  Sn <: Tn
+                  ----------------------------------               (S_RcdDepth)
+                  {i1:S1...in:Sn} <: {i1:T1...in:Tn}
+
+         {i1:S1...in:Sn} is a permutation of {i1:T1...in:Tn}
+         ---------------------------------------------------        (S_RcdPerm)
+                  {i1:S1...in:Sn} <: {i1:T1...in:Tn}
+*)
 
 (** Note that we don't need any special rules for base types: they are
     automatically subtypes of themselves (by [S_Refl]) and [Top] (by
     [S_Top]), and that's all we want. *)
 
-Hint Constructors subtype.
+Hint Constructors well_formed_ty subtype.
 
 Tactic Notation "subtype_cases" tactic(first) ident(c) :=
   first;
   [ Case_aux c "S_Refl" | Case_aux c "S_Trans"
-  | Case_aux c "S_Top" | Case_aux c "S_Arrow" 
+  | Case_aux c "S_Top" | Case_aux c "S_Arrow"
+  | Case_aux c "S_Prod"
+  | Case_aux c "S_RcdWidthBoth"
+  | Case_aux c "S_RcdWidthNil"
+(*  | Case_aux c "S_RcdWidthSub" *)
+  | Case_aux c "S_RcdDepth"
+  | Case_aux c "S_RcdPerm"
+
+(*
+  | Case_aux c "S_ProdWidth1"
+  | Case_aux c "S_ProdWidth2"
+*)
+(*  | Case_aux c "S_ProdPerm" *)
   ].
+
+Lemma has_subtype__wf : forall S T,
+  S <: T ->
+  well_formed_ty S /\ well_formed_ty T.
+Proof with eauto.
+(*  T_cases (induction S) Case; intros; eauto; try solve by inversion. *)
+  (*
+  intros.
+  remember T as rem. generalize dependent T. 
+  subtype_cases (induction H) Case; intros; eauto; try solve by inversion.
+  *)
+  
+  intros.
+  subtype_cases (induction H) Case; eauto; try solve by inversion...
+  inv IHsubtype1... inv IHsubtype2...
+  inv IHsubtype1... inv IHsubtype2...
+  inv IHsubtype1... inv IHsubtype2...
+  inv IHsubtype...
+  inv IHsubtype...
+Qed.
+
+  (*
+Lemma has_type__wf : forall Gamma t T,
+  Gamma |- t \in T -> well_formed_ty T.
+  *)
 
 Module Examples.
 
@@ -777,6 +1563,7 @@ Notation C := (TBase (Id 8)).
 Notation String := (TBase (Id 9)).
 Notation Float := (TBase (Id 10)).
 Notation Integer := (TBase (Id 11)).
+Notation Department := (TBase (Id 12)).
 
 (** **** Exercise: 2 stars, optional (subtyping_judgements) *)
 
@@ -792,30 +1579,106 @@ Notation Integer := (TBase (Id 11)).
                   ssn  : Integer }
 *)
 
+Definition name := (Id 10).
+Notation gpa := (Id 11).
+Notation ssn := (Id 12).
+
 Definition Person : ty := 
-(* FILL IN HERE *) admit.
+  (TRCons name String TRNil).
 Definition Student : ty := 
-(* FILL IN HERE *) admit.
+  (TRCons name String (TRCons gpa Float TRNil)).
+Definition Student' : ty := 
+  (TRCons gpa Float (TRCons name String TRNil)).
 Definition Employee : ty := 
-(* FILL IN HERE *) admit.
+  (TRCons name String (TRCons ssn Integer TRNil)).
+
+Definition perm_xyz : ty :=
+  (TRCons x A (TRCons y B (TRCons z C TRNil))).
+Definition perm_xzy : ty :=
+  (TRCons x A (TRCons z C (TRCons y B TRNil))).
+Definition perm_yxz : ty :=
+  (TRCons y B (TRCons x A (TRCons z C TRNil))).
+Definition perm_yzx : ty :=
+  (TRCons y B (TRCons z C (TRCons x A TRNil))).
+Definition perm_zxy : ty :=
+  (TRCons z C (TRCons x A (TRCons y B TRNil))).
+Definition perm_zyx : ty :=
+  (TRCons z C (TRCons y B (TRCons x A TRNil))).
+
+Example perm_xyz_xyz : 
+  perm_xyz <: perm_xyz.
+Proof with eauto.
+  unfold perm_xyz, perm_xzy, perm_yxz, perm_yzx, perm_zxy, perm_zyx...
+Qed.
+Example perm_xyz_xzy : 
+  perm_xyz <: perm_xzy.
+Proof with eauto.
+  unfold perm_xyz, perm_xzy, perm_yxz, perm_yzx, perm_zxy, perm_zyx. apply S_RcdPerm...
+Qed.
+Example perm_xyz_yxz : 
+  perm_xyz <: perm_yxz.
+Proof with eauto.
+  unfold perm_xyz, perm_xzy, perm_yxz, perm_yzx, perm_zxy, perm_zyx. apply S_RcdPerm...
+Qed.
+Example perm_xyz_yzx : 
+  perm_xyz <: perm_yzx.
+Proof with eauto.
+  unfold perm_xyz, perm_xzy, perm_yxz, perm_yzx, perm_zxy, perm_zyx. apply S_RcdPerm...
+Qed.
+Example perm_xyz_zxy : 
+  perm_xyz <: perm_zxy.
+Proof with eauto.
+  unfold perm_xyz, perm_xzy, perm_yxz, perm_yzx, perm_zxy, perm_zyx. apply S_RcdPerm...
+Qed.
+Example perm_xyz_zyx : 
+  perm_xyz <: perm_zyx.
+Proof with eauto.
+  unfold perm_xyz, perm_xzy, perm_yxz, perm_yzx, perm_zxy, perm_zyx. apply S_RcdPerm...
+Qed.
 
 Example sub_student_person :
   Student <: Person.
-Proof. 
-(* FILL IN HERE *) Admitted.
+Proof.
+  unfold Student, Person.
+  auto.
+Qed.
+
+Example sub_student_student' : 
+  Student <: Student'.
+Proof with eauto.
+  unfold Student', Student. apply S_RcdPerm...
+Qed.
+
+Example sub_student'_student : 
+  Student' <: Student.
+Proof with eauto.
+  unfold Student', Student. apply S_RcdPerm...
+Qed.
+
+Example sub_student'_person :
+  Student' <: Person.
+Proof with eauto.
+  eapply S_Trans.
+  apply sub_student'_student.
+  apply sub_student_person.
+Qed.
 
 Example sub_employee_person :
   Employee <: Person.
-Proof. 
-(* FILL IN HERE *) Admitted.
+Proof.
+  unfold Employee, Person.
+  auto.
+Qed.
 (** [] *)
 
 Example subtyping_example_0 :
   (TArrow C Person) <: (TArrow C TTop).
   (* C->Person <: C->Top *)
 Proof.
+  unfold Person.
   apply S_Arrow.
     apply S_Refl. auto.
+    apply S_Top. eauto.
 Qed.
 
 (** The following facts are mostly easy to prove in Coq.  To get
@@ -827,7 +1690,14 @@ Example subtyping_example_1 :
   (TArrow TTop Student) <: (TArrow (TArrow C C) Person).
   (* Top->Student <: (C->C)->Person *)
 Proof with eauto.
-  (* FILL IN HERE *) Admitted.
+  unfold Student, Person.
+  eapply S_Arrow.
+  apply S_Top.
+
+
+  auto.
+  apply sub_student_person.
+Qed.
 (** [] *)
 
 (** **** Exercise: 1 star, optional (subtyping_example_2) *)
@@ -835,8 +1705,9 @@ Example subtyping_example_2 :
   (TArrow TTop Person) <: (TArrow Person TTop).
   (* Top->Person <: Person->Top *)
 Proof with eauto.
-  (* FILL IN HERE *) Admitted.
-(** [] *)
+  unfold Person.
+  auto.
+Qed.
 
 End Examples.
 
@@ -858,8 +1729,10 @@ Inductive has_type : context -> tm -> ty -> Prop :=
   (* Same as before *)
   | T_Var : forall Gamma x T,
       Gamma x = Some T ->
+      well_formed_ty T ->
       Gamma |- (tvar x) \in T
   | T_Abs : forall Gamma x T11 T12 t12,
+      well_formed_ty T11 ->
       (extend Gamma x T11) |- t12 \in T12 -> 
       Gamma |- (tabs x T11 t12) \in (TArrow T11 T12)
   | T_App : forall T1 T2 Gamma t1 t2,
@@ -879,10 +1752,34 @@ Inductive has_type : context -> tm -> ty -> Prop :=
       Gamma |- tunit \in TUnit
   (* New rule of subsumption *)
   | T_Sub : forall Gamma t S T,
+      well_formed_ty T ->
       Gamma |- t \in S ->
       S <: T ->
       Gamma |- t \in T
 
+  | T_Pair : forall Gamma t1 t2 T1 T2,
+      Gamma |- t1 \in T1 ->
+      Gamma |- t2 \in T2 ->
+      Gamma |- (tpair t1 t2) \in (TProd T1 T2)
+  | T_Fst : forall Gamma t T1 T2,
+      Gamma |- t \in (TProd T1 T2) ->
+      Gamma |- (tfst t) \in T1
+  | T_Snd : forall Gamma t T1 T2,
+      Gamma |- t \in (TProd T1 T2) ->
+      Gamma |- (tsnd t) \in T2                       
+
+  | T_Proj : forall Gamma i t Ti Tr,
+      Gamma |- t \in Tr ->
+      Tlookup i Tr = Some Ti ->
+      Gamma |- (tproj t i) \in Ti
+  | T_RNil : forall Gamma,
+      Gamma |- trnil \in TRNil
+  | T_RCons : forall Gamma i t T tr Tr,
+      Gamma |- t \in T ->
+      Gamma |- tr \in Tr ->
+      record_ty Tr ->
+      record_tm tr ->
+      Gamma |- (trcons i t tr) \in (TRCons i T Tr)                              
 where "Gamma '|-' t '\in' T" := (has_type Gamma t T).
 
 Hint Constructors has_type.
@@ -893,7 +1790,174 @@ Tactic Notation "has_type_cases" tactic(first) ident(c) :=
   | Case_aux c "T_App" | Case_aux c "T_True" 
   | Case_aux c "T_False" | Case_aux c "T_If"
   | Case_aux c "T_Unit"     
-  | Case_aux c "T_Sub" ].
+  | Case_aux c "T_Sub"
+  | Case_aux c "T_Pair"
+  | Case_aux c "T_Fst"
+  | Case_aux c "T_Snd"
+  | Case_aux c "T_Proj"
+  | Case_aux c "T_RNil"
+  | Case_aux c "T_RCons"
+  ].
+
+
+
+
+
+
+
+
+
+
+
+
+
+
+
+
+Lemma wf_rcd_lookup : forall i T Ti,
+  well_formed_ty T ->
+  Tlookup i T = Some Ti ->
+  well_formed_ty Ti.
+Proof with eauto.
+  intros i T.
+  T_cases (induction T) Case; intros; try solve by inversion.
+  Case "TRCons".
+    inversion H. subst. unfold Tlookup in H0.
+    destruct (eq_id_dec i i0)...
+    inversion H0. subst...  Qed.
+
+Lemma step_preserves_record_tm : forall tr tr',
+  record_tm tr ->
+  tr ==> tr' ->
+  record_tm tr'.
+Proof.
+  intros tr tr' Hrt Hstp.
+  inversion Hrt; subst; inversion Hstp; subst; auto.
+Qed.
+
+Lemma has_type__wf : forall Gamma t T,
+  Gamma |- t \in T -> well_formed_ty T.
+Proof with eauto.
+  intros Gamma t T Htyp.
+  has_type_cases (induction Htyp) Case; eauto; try solve by inversion...
+  Case "T_App".
+    inversion IHHtyp1...
+  Case "T_Fst".
+    inv IHHtyp...
+  Case "T_Snd".
+    inv IHHtyp...
+  Case "T_Proj".
+    eapply wf_rcd_lookup...
+Qed.
+
+Lemma lookup_in_sublist : forall Ti T1 T2 i,
+  is_sublist T2 T1 ->
+  Tlookup i T2 = Some Ti ->
+  Tlookup i T1 = Some Ti.
+Proof with eauto.
+  intros.
+  generalize dependent i.
+  induction H; intros. inv H0.
+  inv H1...
+  destruct (eq_id_dec i0 i). subst...
+  generalize H3; intro.
+  apply IHis_sublist in H1.
+  rewrite H1. rewrite H3. reflexivity.
+Qed.
+
+Lemma lookup_in_subtype : forall S T i T1,
+(*  well_formed_ty T -> *)
+  S <: T ->
+  Tlookup i T = Some T1 ->
+(*  Tlookup i S = Some T1. *)
+  exists T2, (Tlookup i S = Some T2) /\ (T2 <: T1).
+Proof with eauto.
+  intros.
+  generalize dependent T1.
+  generalize dependent i.
+  subtype_cases (induction H) Case; intros; eauto; try solve by inversion...
+  Case "S_Refl". exists T1... split... eapply wf_rcd_lookup in H...
+  Case "S_Trans".
+  generalize (IHsubtype2 i T1); intro Tmp; exploit Tmp; eauto; intro; clear Tmp.
+  inv H2. inv H3.
+  generalize (IHsubtype1 i x); intro Tmp; exploit Tmp; eauto; intro; clear Tmp.
+  inv H3. inv H5.
+  eexists; eauto.
+  Case "S_RcdWidthBoth".
+  destruct (eq_id_dec i i0); inv H3; simpl in *.
+  repeat rewrite eq_id in *... inv H5. exists T0...
+  rewrite neq_id in *...
+(*
+  destruct (eq_id_dec i i0); inv H2; simpl in *. repeat rewrite eq_id in *...
+  rewrite neq_id in *...   rewrite neq_id in *...
+  generalize (IHsubtype i0 Ti0); intro T; exploit T; eauto; intro; clear T.
+  rewrite H4. rewrite H2...
+*)
+  Case "S_RcdDepth".
+  simpl in *.
+  destruct (eq_id_dec i0 i)... inv H2...
+  eapply wf_rcd_lookup in H...
+  Case "S_RcdPerm".
+  exists T0; split...
+  eapply lookup_in_sublist...
+  eapply wf_rcd_lookup in H0...
+(*  
+  inv H2... inv H3...
+  repeat simpl in *.
+  destruct (eq_id_dec i i0). subst... inv H3...
+  inv H4... inv H3...
+  destruct (eq_id_dec i i1). subst... simpl in H3. rewrite eq_id in H3... inv H3...
+  simpl in H3. rewrite neq_id in H3...
+  
+  inv H1... inv H2... inv H4...
+  inv H... eexists T0; split...
+  inv H0; intros; eauto; try solve by inversion.
+(*  induction H0; intros; eauto; try solve by inversion. *)
+  inv H2...
+
+  
+  inv H3...
+  destruct (eq_id_dec i i0)... subst...
+  simpl in H8. rewrite neq_id in H8... simpl.
+  destruct (eq_id_dec i i1)... subst... inv H5. rewrite neq_id in *...
+  destruct (eq_id_dec i0 i1)... subst... simpl in H5. rewrite eq_id in H5...
+  admit. admit. admit.
+*)
+Qed.
+
+Lemma lookup_field_in_value : forall v T i Ti,
+  value v ->
+  empty |- v \in T ->
+  Tlookup i T = Some Ti ->
+(*  exists ti, tlookup i v = Some ti /\ empty |- ti \in Ti. *)
+  exists ti S, tlookup i v = Some ti /\ empty |- ti \in S /\ S <: Ti.
+Proof with eauto.
+  intros v T i Ti Hval Htyp Hget.
+  remember empty as Gamma.
+  generalize dependent Ti.
+  has_type_cases (induction Htyp) Case; intros; subst; try solve by inversion...
+  Case "T_Sub".
+    generalize H0; intro.
+    eapply lookup_in_subtype in H0... inv H0. inv H2.
+    edestruct (IHHtyp Hval)... inv H2... inv H4. inv H5.
+    exists x0. exists x1. eauto.
+  Case "T_RCons".
+    simpl in Hget. simpl. destruct (eq_id_dec i i0).
+    SCase "i is first".
+      simpl. inversion Hget. subst.
+      exists t... exists Ti... split... split... apply has_type__wf in Htyp1...
+    SCase "get tail".
+      apply IHHtyp2... inv Hval...
+(*      destruct IHHtyp2 as [vi [Hgeti Htypi]]...
+      inversion Hval... Qed.
+*)
+Qed.
+
+
+
+
+
+
 
 (* ############################################### *)
 (** ** Typing examples *)
@@ -908,20 +1972,63 @@ Import Examples.
 (** **** Exercise: 1 star, optional (typing_example_0) *)
 (* empty |- ((\z:A.z), (\z:B.z)) 
           : (A->A * B->B) *)
-(* FILL IN HERE *)
-(** [] *)
+Example typing_example_0 : forall A B,
+  well_formed_ty A ->
+  well_formed_ty B ->
+  empty |- (tpair (tabs z A (tvar z)) (tabs z B (tvar z))) \in (TProd (TArrow A A) (TArrow B B)).
+Proof with eauto.
+  intros...
+  apply T_Pair...
+Qed.
 
 (** **** Exercise: 2 stars, optional (typing_example_1) *)
 (* empty |- (\x:(Top * B->B). x.snd) ((\z:A.z), (\z:B.z)) 
           : B->B *)
-(* FILL IN HERE *)
+Example typing_example_1 : forall A B,
+  well_formed_ty A ->
+  well_formed_ty B ->
+  empty |- (tapp (tabs x (TProd TTop (TArrow B B)) (tsnd (tvar x))) (tpair (tabs z A (tvar z)) (tabs z B (tvar z)))) \in (TArrow B B).
+Proof with eauto.
+  intros...
+  eapply T_App. 
+  eapply T_Abs...
+
+  eapply T_Pair.
+  eapply T_Sub...
+  eapply T_Abs...
+Qed.
 (** [] *)
 
 (** **** Exercise: 2 stars, optional (typing_example_2) *)
 (* empty |- (\z:(C->C)->(Top * B->B). (z (\x:C.x)).snd)
               (\z:C->C. ((\z:A.z), (\z:B.z)))
           : B->B *)
-(* FILL IN HERE *)
+Example typing_example_2 : forall A B C,
+  well_formed_ty A ->
+  well_formed_ty B ->
+  well_formed_ty C ->
+  empty |- (tapp (tabs z (TArrow (TArrow C C) (TProd TTop (TArrow B B)))
+                 (tsnd (tapp (tvar z) (tabs x C (tvar x)))))
+                 (tabs z (TArrow C C)
+                       (tpair
+                          (tabs z A (tvar z))
+                          (tabs z B (tvar z))
+                       )
+                 )
+           ) \in (TArrow B B).
+Proof with eauto.
+  intros...
+  eapply T_App.
+  eapply T_Abs...
+  eapply T_Snd.
+  eapply T_App. eapply T_Var...
+  eapply T_Abs...
+  eapply T_Abs...
+  eapply T_Pair.
+  eapply T_Sub...
+  eapply T_Abs...
+Qed.
+
 (** [] *)
 
 End Examples2.
@@ -959,7 +2066,37 @@ Lemma sub_inversion_Bool : forall U,
 Proof with auto.
   intros U Hs.
   remember TBool as V.
-  (* FILL IN HERE *) Admitted.
+
+  induction Hs; inv HeqV...
+  apply IHHs2 in H. apply IHHs1 in H. subst. apply IHHs2...
+  inv H0.
+(*  inv H0. *)
+  inv H3... inv H4...
+  inv H6...
+Qed.
+
+Lemma sub_inversion_Top : forall T,
+     TTop <: T ->
+     T = TTop.
+Proof with eauto.
+  intros.
+  remember (TTop) as rem.
+  subtype_cases (induction H) Case; subst; simpl; eauto; try solve by inversion.
+  exploit IHsubtype1; eauto; intro; subst...
+Qed.
+
+(*
+Lemma sub_inversion_Unit : forall T,
+     TUnit <: T ->
+     T = TUnit.
+Proof.
+  intros.
+  remember (TUnit) as rem.
+  subtype_cases (induction H) Case; subst; simpl; eauto; try solve by inversion.
+  exploit IHsubtype1; eauto; intro; subst...
+Qed.
+*)
+
 
 (** **** Exercise: 3 stars, optional (sub_inversion_arrow) *)
 Lemma sub_inversion_arrow : forall U V1 V2,
@@ -970,7 +2107,40 @@ Proof with eauto.
   intros U V1 V2 Hs.
   remember (TArrow V1 V2) as V.
   generalize dependent V2. generalize dependent V1.
-  (* FILL IN HERE *) Admitted.
+
+  subtype_cases (induction Hs) Case; intros; subst; try solve by inversion.
+  inv H...
+  exists V1; exists V2... 
+
+  assert(G : S <: TArrow V1 V2) by eauto.
+  generalize (IHHs2 V1 V2); intros T; exploit T; eauto; intro; clear T.
+  inv H... inv H0... inv H. inv H1.
+  generalize (IHHs1 x x0); intros T; exploit T; eauto; intro; clear T.
+  inv H1. inv H2. inv H1. inv H3.
+  exists x1; exists x2...
+  inv HeqV...
+Qed.
+
+
+Lemma sub_inversion_prod : forall U V1 V2,
+     U <: (TProd V1 V2) ->
+     exists U1, exists U2, 
+       U = (TProd U1 U2) /\ (U1 <: V1) /\ (U2 <: V2).
+Proof with eauto.
+  intros.
+  remember (TProd V1 V2) as V.
+  generalize dependent V2. generalize dependent V1.
+  subtype_cases (induction H) Case; intros; subst; simpl; try solve by inversion.
+  Case "S_Refl".
+  inv H...
+  exists V1; exists V2...
+  edestruct IHsubtype2... inv H1. inv H2. inv H3.
+  edestruct IHsubtype1... inv H3. inv H4. inv H5.
+  exists x1; exists x2...
+  Case "S_Prod".
+  inv HeqV.
+  inv H0; eexists... (* ???????????????? MAGIC????????????????? *)
+Qed.
 
 
 (** [] *)
@@ -1008,7 +2178,19 @@ Lemma canonical_forms_of_arrow_types : forall Gamma s T1 T2,
   exists x, exists S1, exists s2,
      s = tabs x S1 s2.
 Proof with eauto.
-  (* FILL IN HERE *) Admitted.
+(*  
+  t_cases (induction s) Case; intros; try solve by inversion.
+  inv H...
+  inv H... inv H1...
+*)
+  intros.
+  remember (TArrow T1 T2) as T.
+  generalize dependent T1.
+  generalize dependent T2.
+  induction H; intros; subst; simpl; eauto; try solve by inversion.
+  apply sub_inversion_arrow in H2. inv H2. inv H3. inv H2.
+  generalize (IHhas_type H0 x0 x); intro T; exploit T...
+Qed.
 (** [] *)
 
 (** Similarly, the canonical forms of type [Bool] are the constants
@@ -1023,7 +2205,48 @@ Proof with eauto.
   remember TBool as T.
   has_type_cases (induction Hty) Case; try solve by inversion...
   Case "T_Sub".
-    subst. apply sub_inversion_Bool in H. subst...
+    subst. apply sub_inversion_Bool in H0. subst...
+Qed.
+
+(*
+Lemma canonical_forms_of_pair_types : forall Gamma s T1 T2,
+  Gamma |- s \in (TProd T1 T2) ->
+  value s ->
+  exists x y, s = (tpair x y).
+*)
+Lemma canonical_forms_of_pair_types : forall s T1 T2,
+  empty |- s \in (TProd T1 T2) ->
+  value s ->
+  exists x y, s = (tpair x y).
+Proof with eauto.
+  intros.
+  remember (empty) as Gamma.
+  remember (TProd T1 T2) as rem.
+  generalize dependent T1.
+  generalize dependent T2.
+  has_type_cases (induction H) Case; intros; subst; simpl; eauto; try solve by inversion...
+  Case "T_Sub".
+(*  
+  remember (TProd T1 T2) as rem.
+  clear IHhas_type. 
+  subtype_cases (induction H2) SCase; subst; simpl; eauto; try solve by inversion...
+  SCase "S_Refl". 
+  SCase "S_Trans". admit.
+  SCase "S_Prod". 
+*)
+  generalize H2; intro.
+  apply sub_inversion_prod in H2. inv H2. inv H4. inv H2. inv H5. 
+  subst...
+  (*
+  remember (empty) as Gamma.
+  remember (TProd x x0) as rem.
+  has_type_cases (induction H1) SCase; subst; simpl; eauto; try solve by inversion...
+  
+  inv H1. inv H5. inv H0. inv H0. admit.
+  inv H0. exists t1; exists t2...
+  inv H0. inv H0.
+  inv H0.
+*)
 Qed.
 
 
@@ -1117,6 +2340,33 @@ Proof with eauto.
       inversion H0; subst...
       inversion H. rename x into t1'. eauto.
 
+  Case "T_Pair".
+    destruct IHHt1; destruct IHHt2...
+(*    exploit IHHt1; eauto; intro. exploit IHHt2; eauto; intro. *)
+    inv H; inv H0...
+    inv H. right. eexists...
+    inv H. right. eexists...
+  Case "T_Fst".
+    destruct IHHt...
+    apply canonical_forms_of_pair_types in Ht... inv Ht. inv H0. inv H.
+    right. eexists...
+    inv H. right. eexists... 
+  Case "T_Snd".
+    destruct IHHt...
+    apply canonical_forms_of_pair_types in Ht... inv Ht. inv H0. inv H.
+    right. eexists...
+    inv H. right. eexists... 
+  Case "T_Proj".
+    destruct IHHt...
+    right.
+    apply lookup_field_in_value with (v:=t) in H... inv H. inv H1. inv H. inv H2.
+    eexists...
+    inv H0. right. eexists...
+  Case "T_RCons".
+    destruct IHHt1; destruct IHHt2...
+    inv H2. right. eexists...
+    inv H1. right. eexists...
+    inv H1; inv H2. right. eexists...
 Qed.
 
 (* ########################################## *)
@@ -1169,7 +2419,7 @@ Proof with eauto.
   has_type_cases (induction H) Case; 
     inversion Heqt; subst; intros; try solve by inversion.
   Case "T_Abs".
-    exists T12...
+    exists T12... split... apply S_Refl... econstructor... apply has_type__wf in H0...
   Case "T_Sub".
     destruct IHhas_type as [S2 [Hsub Hty]]...
   Qed.
@@ -1203,7 +2453,12 @@ Proof with eauto.
   Case "T_App".
     exists T1...
   Case "T_Sub".
+(*    provided script broken *)  
+(*    destruct IHHty as [U1 [Hty1 Hty2]]... *)
     destruct IHHty as [U1 [Hty1 Hty2]]...
+    exists U1. split... apply T_Sub with (S:=(TArrow U1 S))...
+    econstructor... apply has_type__wf in Hty2...
+    eapply S_Arrow... eapply has_type__wf in Hty2... 
 Qed.
 
 Lemma typing_inversion_true : forall Gamma T,
@@ -1237,7 +2492,11 @@ Proof with eauto.
   Case "T_If".
     auto.
   Case "T_Sub".
-    destruct (IHHty H0) as [H1 [H2 H3]]...
+(*    provided script broken *)
+(*    destruct (IHHty H0) as [H1 [H2 H3]]... *)
+  destruct IHHty... 
+  inv H3.
+  split...
 Qed.
 
 Lemma typing_inversion_unit : forall Gamma T,
@@ -1249,6 +2508,128 @@ Proof with eauto.
     inversion Heqtu; subst; intros...
 Qed.
 
+Lemma typing_inversion_pair : forall Gamma t1 t2 T,
+  Gamma |- tpair t1 t2 \in T ->
+  (exists S1 S2,
+    Gamma |- t1 \in S1 /\
+    Gamma |- t2 \in S2
+(* below is crucial *)
+                    /\
+    TProd S1 S2 <: T
+  ).
+                           (*
+  exists T1 T2, T = TProd T1 T2 /\
+  (exists S1 S2,
+    Gamma |- t1 \in S1 /\
+    Gamma |- t2 \in S2)
+.
+*)
+Proof with eauto.
+  intros Gamma t1 t2 T Htyp. remember (tpair t1 t2) as tu.
+  has_type_cases (induction Htyp) Case;
+    inversion Heqtu; subst; intros...
+  (*
+  clear H1. destruct IHHtyp... inv H1... inv H2... inv H3... inv H1... inv H2...
+  eexists
+*)
+  destruct IHHtyp... clear H1.
+  inv H2. inv H1. inv H3.
+  exists x; exists x0...
+
+  exists T1; exists T2... split... split...
+  apply S_Refl. apply has_type__wf in Htyp2. apply has_type__wf in Htyp1...
+Qed.
+(*  
+Lemma typing_inversion_pair : forall Gamma t1 t2 T,
+  Gamma |- tpair t1 t2 \in T ->
+  exists T1 T2, Gamma |- tpair t1 t2 \in TProd T1 T2.
+Proof with eauto.
+  intros Gamma t1 t2 T Htyp. remember (tpair t1 t2) as tu.
+  has_type_cases (induction Htyp) Case;
+    inversion Heqtu; subst; intros...  
+Qed.
+*)
+
+Lemma typing_inversion_fst : forall Gamma t T,
+  Gamma |- tfst t \in T ->
+  (exists S1 S2,
+    Gamma |- t \in (TProd S1 S2) /\
+    S1 <: T
+  ).  
+Proof with eauto.
+  intros Gamma t T Htyp. remember (tfst t) as rem.
+  has_type_cases (induction Htyp) Case;
+    inversion Heqrem; subst; intros...
+  clear H1. destruct IHHtyp... inv H1. inv H2.
+  exists x; exists x0...
+
+  exists T1; exists T2; split...
+  apply has_type__wf in Htyp; inv Htyp...
+Qed.
+
+Lemma typing_inversion_snd : forall Gamma t T,
+  Gamma |- tsnd t \in T ->
+  (exists S1 S2,
+    Gamma |- t \in (TProd S1 S2) /\
+    S2 <: T
+  ).  
+Proof with eauto.
+  intros Gamma t T Htyp. remember (tsnd t) as rem.
+  has_type_cases (induction Htyp) Case;
+    inversion Heqrem; subst; intros...
+  clear H1. destruct IHHtyp... inv H1. inv H2.
+  exists x; exists x0...
+
+  exists T1; exists T2; split...
+  apply has_type__wf in Htyp; inv Htyp...
+Qed.
+
+Lemma typing_inversion_tproj : forall Gamma tr i Ti,
+  Gamma |- tproj tr i \in Ti ->
+  exists Tr S,
+    Tlookup i Tr = Some S /\
+    S <: Ti /\
+    Gamma |- tr \in Tr.
+Proof with eauto.
+  intros Gamma tr i Ti Htyp. remember (tproj tr i) as rem.
+  has_type_cases (induction Htyp) Case;
+    inversion Heqrem; subst; intros...
+  destruct IHHtyp...
+  inv H2. inv H3. inv H4.
+  exists x; exists x0; split... 
+
+  exists Tr; exists Ti; split... split...
+  apply wf_rcd_lookup in H... apply has_type__wf in Htyp...
+Qed.
+
+Lemma typing_inversion_trnil : forall Gamma T,
+  Gamma |- trnil \in T ->
+  TRNil <: T.
+Proof with eauto.
+  intros Gamma T Htyp. remember (trnil) as rem.
+  has_type_cases (induction Htyp) Case;
+    inversion Heqrem; subst; intros...
+Qed.
+
+Lemma typing_inversion_trcons : forall Gamma i t tr U,
+  Gamma |- trcons i t tr \in U ->
+  (exists T Tr,
+    Gamma |- t \in T /\
+    Gamma |- tr \in Tr /\
+    record_ty Tr /\
+    record_tm tr /\
+    TRCons i T Tr <: U).
+Proof with eauto.
+  intros Gamma i t tr U Htyp. remember (trcons i t tr) as rem.
+  has_type_cases (induction Htyp) Case;
+    inversion Heqrem; subst; intros...
+  destruct IHHtyp... inv H2. inv H3. inv H4. inv H5. inv H6.
+  exists x; exists x0... split...
+  exists T; exists Tr... split... split... split... split... apply S_Refl.
+  constructor...
+  apply has_type__wf in Htyp1...
+  apply has_type__wf in Htyp2...
+Qed.
 
 (** The inversion lemmas for typing and for subtyping between arrow
     types can be packaged up as a useful "combination lemma" telling
@@ -1264,7 +2645,23 @@ Proof with eauto.
   inversion Hty as [S2 [Hsub Hty1]].
   apply sub_inversion_arrow in Hsub.
   inversion Hsub as [U1 [U2 [Heq [Hsub1 Hsub2]]]].
-  inversion Heq; subst...  Qed.
+  inversion Heq; subst...
+  (* provided script broken *)
+  split... (* apply T_Sub with (S:=U2)... *) eapply T_Sub...
+  apply has_subtype__wf in Hsub2. inv Hsub2...
+  (*
+  inv Hty. inv Hsub. inv H0. inv H1. inv H. inv H2.
+  admit.
+*)
+(*  
+has_type__wf:
+  forall (Gamma : context) (t : tm) (T : ty),
+  Gamma |- t \in T -> well_formed_ty T
+wf_rcd_lookup:
+  forall (i : id) (T Ti : ty),
+  well_formed_ty T -> Tlookup i T = Some Ti -> well_formed_ty Ti
+*)
+Qed.
 
 (* ########################################## *)
 (** ** Context Invariance *)
@@ -1292,6 +2689,32 @@ Inductive appears_free_in : id -> tm -> Prop :=
   | afi_if3 : forall x t1 t2 t3,
       appears_free_in x t3 ->
       appears_free_in x (tif t1 t2 t3)
+  | afi_pair1 : forall x t1 t2,
+      appears_free_in x t1 ->
+      appears_free_in x (tpair t1 t2)
+  | afi_pair2 : forall x t1 t2,
+      appears_free_in x t2 ->
+      appears_free_in x (tpair t1 t2)
+  | afi_fst : forall x t,
+      appears_free_in x t ->
+      appears_free_in x (tfst t)
+  | afi_snd : forall x t,
+      appears_free_in x t ->
+      appears_free_in x (tsnd t)
+  | afi_proj : forall x tr i,
+      appears_free_in x tr ->
+      appears_free_in x (tproj tr i)
+(*
+  | afi_rcons_new : forall x i t tr,
+      appears_free_in x t ->
+      appears_free_in x (trcons i t tr)
+  | afi_rcons_already : forall x i t tr,
+      appears_free_in x tr ->
+      appears_free_in x (trcons i t tr)
+*)
+  | afi_rcons : forall x i t tr,
+      appears_free_in x tr \/ appears_free_in x t ->
+      appears_free_in x (trcons i t tr)
 .
 
 Hint Constructors appears_free_in.
@@ -1314,7 +2737,10 @@ Proof with eauto.
     apply T_App with T1...
   Case "T_If".
     apply T_If...
-
+  Case "T_Pair".
+    apply T_Pair...
+  Case "T_RCons".
+    apply T_RCons... 
 Qed.
 
 Lemma free_in_context : forall x t T Gamma,
@@ -1326,8 +2752,13 @@ Proof with eauto.
   has_type_cases (induction Htyp) Case; 
       subst; inversion Hafi; subst...
   Case "T_Abs".
-    destruct (IHHtyp H4) as [T Hctx]. exists T.
-    unfold extend in Hctx. rewrite neq_id in Hctx...  Qed.
+(*    destruct (IHHtyp H4) as [T Hctx]. exists T. *)  
+    destruct (IHHtyp H5) as [T Hctx]. exists T.
+    unfold extend in Hctx. rewrite neq_id in Hctx...
+(* provided  script broken *)
+  Case "T_RCons".
+    inv H3. eapply IHHtyp2... eapply IHHtyp1...
+Qed.
 
 (* ########################################## *)
 (** ** Substitution *)
@@ -1339,11 +2770,104 @@ Proof with eauto.
     extract structural information from assumptions about the
     well-typedness of subterms. *)
 
+
+(*
+Lemma extend_var_subtype : forall Gamma S x U y,
+  extend Gamma x U |- tvar y \in S ->
+  x <> y ->
+  Gamma |- tvar y \in S.
+Proof with eauto.
+  intros.
+
+  remember (Gamma) as gam.
+  generalize dependent Gamma.
+
+  has_type_cases (induction H) Case; intros; try solve by inversion.
+  apply T_Var...
+Abort.
+*)
+
+
+(*
+  S : ty
+  Htypt : extend Gamma x U |- tvar y \in S
+  T : ty
+  n : x <> y
+  Hctx : Gamma y = Some T
+  Hsub : T <: S
+  ============================
+   Gamma |- tvar y \in S
+*)
+
+(*
+Lemma has_type__wf_abs : forall S Gamma x T t,
+  Gamma |- tabs x T t \in S ->
+  well_formed_ty T.
+Proof with eauto.
+  induction S; intros; try solve by inversion.
+
+  intros.
+  (*
+  remember Gamma as gam.
+  generalize dependent Gamma.
+*)
+(*
+  remember (tabs x T t) as tm.
+  generalize dependent x.
+  generalize dependent T.
+  generalize dependent t.
+*)
+  has_type_cases (induction H) Case; intros;
+  subst; eauto; try solve by inversion.
+
+  inv Heqtm.
+Qed.
+*)
+
+(*
+  Case := "tabs" : String.string
+  x : id
+  U : ty
+  v : tm
+  y : id
+  T1 : ty
+  t0 : tm
+  Htypv : empty |- v \in U
+  IHt : forall (Gamma : context) (S : ty),
+        extend Gamma x U |- t0 \in S -> Gamma |- [x := v]t0 \in S
+  Gamma : context
+  S : ty
+  Htypt : extend Gamma x U |- tabs y T1 t0 \in S
+  T2 : ty
+  Hsub : TArrow T1 T2 <: S
+  Htypt2 : extend (extend Gamma x U) y T1 |- t0 \in T2
+  ============================
+   well_formed_ty T1
+
+
+     : forall (Gamma : context) (t : tm) (T : ty),
+       Gamma |- t \in T -> well_formed_ty T
+
+T_Abs:
+  forall (Gamma : context) (x : id) (T11 T12 : ty) (t12 : tm),
+  well_formed_ty T11 ->
+  extend Gamma x T11 |- t12 \in T12 ->
+  Gamma |- tabs x T11 t12 \in TArrow T11 T12
+*)
+
+
+Lemma subst_keeps_record_tm : forall x v t,
+  record_tm t ->
+  record_tm ([x := v] t).
+Proof with eauto.
+  induction t; intros; simpl; eauto; try solve by inversion...
+Qed.
+
 Lemma substitution_preserves_typing : forall Gamma x U v t S,
      (extend Gamma x U) |- t \in S  ->
      empty |- v \in U   ->
      Gamma |- ([x:=v]t) \in S.
-Proof with eauto.
+Proof with eauto. (* using has_type__wf, has_subtype__wf.  too slow*)
   intros Gamma x U v t S Htypt Htypv.
   generalize dependent S. generalize dependent Gamma.
   t_cases (induction t) Case; intros; simpl.
@@ -1357,10 +2881,29 @@ Proof with eauto.
       subst.
       inversion Hctx; subst. clear Hctx.
       apply context_invariance with empty...
+      (* provided script broken *)
+      eapply T_Sub... apply has_type__wf in Htypt... 
       intros x Hcontra.
       destruct (free_in_context _ _ S empty Hcontra) 
           as [T' HT']...
+      (* provided script broken *)
+      eapply T_Sub... apply has_type__wf in Htypt... 
       inversion HT'.
+    SCase "x<>y".
+      apply T_Sub with (T)... apply has_subtype__wf in Hsub. inv Hsub...
+      econstructor... apply has_subtype__wf in Hsub. inv Hsub...
+(*      
+      generalize Htypt; intro G.
+      apply typing_inversion_var in G. inv G. inv H.
+      unfold extend in H0. rewrite neq_id in H0...
+
+      rewrite Hctx in H0. inv H0...
+      
+      inv Htypt. unfold extend in H0. rewrite neq_id in H0...
+      apply T_Sub with (S0)... inv H0.
+      unfold extend in H3. rewrite neq_id in H3...
+*)
+
   Case "tapp".
     destruct (typing_inversion_app _ _ _ _ Htypt) 
         as [T1 [Htypt1 Htypt2]].
@@ -1369,7 +2912,21 @@ Proof with eauto.
     rename i into y. rename t into T1.
     destruct (typing_inversion_abs _ _ _ _ _ Htypt) 
       as [T2 [Hsub Htypt2]].
-    apply T_Sub with (TArrow T1 T2)... apply T_Abs...
+    apply T_Sub with (TArrow T1 T2)... apply has_type__wf in Htypt...
+    apply T_Abs...
+    apply has_subtype__wf in Hsub. inv Hsub. inv H...
+
+(*
+    apply canonical_forms_of_arrow_types in Hsub.
+    
+     : forall (s : tm) (T1 T2 : ty),
+       empty |- s \in TProd T1 T2 ->
+       value s -> exists x y : tm, s = tpair x y
+
+       U <: TArrow V1 V2 ->
+       exists U1 U2 : ty, U = TArrow U1 U2 /\ V1 <: U1 /\ U2 <: V2
+*)
+                                                                  
     destruct (eq_id_dec x y).
     SCase "x=y".
       eapply context_invariance...
@@ -1384,9 +2941,11 @@ Proof with eauto.
   Case "ttrue".
       assert (TBool <: S) 
         by apply (typing_inversion_true _ _  Htypt)...
+      eapply T_Sub... apply has_type__wf in Htypt... 
   Case "tfalse".
       assert (TBool <: S) 
         by apply (typing_inversion_false _ _  Htypt)...
+      eapply T_Sub... apply has_type__wf in Htypt... 
   Case "tif".
     assert ((extend Gamma x U) |- t1 \in TBool 
             /\ (extend Gamma x U) |- t2 \in S
@@ -1398,6 +2957,53 @@ Proof with eauto.
   Case "tunit".
     assert (TUnit <: S) 
       by apply (typing_inversion_unit _ _  Htypt)...
+    inv Htypt...
+  Case "tpair".
+    generalize Htypt; intro G.
+    apply typing_inversion_pair in G.
+    inv G. inv H. inv H0. inv H1.
+
+    apply IHt1 in H. apply IHt2 in H0.
+    inv Htypt...
+(*             
+    apply has_type__wf in Htypt.
+    inv H0. inv H1. inv H3. inv H5.
+
+       empty |- s \in TProd T1 T2 ->
+       value s -> exists x y : tm, s = tpair x y    
+    econstructor. auto.
+    eapply T_Pair...
+    econstructor...
+*)
+  Case "tfst".
+    generalize Htypt; intro G.
+    apply typing_inversion_fst in G.
+    inv G. inv H. inv H0.
+    inv Htypt...
+  Case "tsnd".
+    generalize Htypt; intro G.
+    apply typing_inversion_snd in G.
+    inv G. inv H. inv H0.
+    inv Htypt...
+  Case "tproj".
+    generalize Htypt; intro G.
+    apply typing_inversion_tproj in G.
+    inv G. inv H. inv H0. inv H1.
+    econstructor...
+    apply has_type__wf in Htypt...
+  Case "trnil".
+    generalize Htypt; intro G.
+    apply typing_inversion_trnil in G.
+    econstructor... apply has_type__wf in Htypt...
+  Case "trcons".
+    generalize Htypt; intro G.
+    apply typing_inversion_trcons in G.
+    inv G. inv H. inv H0. inv H1. inv H2. inv H3.
+    econstructor. apply has_subtype__wf in H4... inv H4...
+    constructor...
+    generalize (IHt2 Gamma x1 H0); intro G.
+    eapply subst_keeps_record_tm in H2...
+    auto.
 Qed.
 
 (* ########################################## *)
@@ -1459,6 +3065,73 @@ Qed.
        result is immediate by the induction hypothesis for the typing
        subderivation and an application of [T_Sub].  [] *)
 
+(*
+  Case := "T_Fst" : String.string
+  T1 : ty
+  T2 : ty
+  t' : tm
+  v2 : tm
+  H0 : value t'
+  H1 : value v2
+  HE : tfst (tpair t' v2) ==> t'
+  IHHT : forall t'0 : tm,
+         empty = empty -> tpair t' v2 ==> t'0 -> empty |- t'0 \in TProd T1 T2
+  S : ty
+  H : well_formed_ty (TProd T1 T2)
+  H3 : S <: TProd T1 T2
+  x : ty
+  x0 : ty
+  H4 : empty |- t' \in x
+  H2 : empty |- v2 \in x0
+  H6 : TProd x x0 <: S
+  G : TProd x x0 <: TProd T1 T2
+  ============================
+   empty |- t' \in T1
+*)
+
+Lemma prod_order : forall T1 T2 U1 U2,
+(*
+  TProd T1 T2 <: TProd U1 U2 ->
+  T1 <: U1 /\ T2 <: U2.
+*)
+  well_formed_ty (TProd T1 T2) ->
+  well_formed_ty (TProd U1 U2) ->
+  TProd T1 T2 <: TProd U1 U2 ->
+  T1 <: U1 /\ T2 <: U2.
+Proof with eauto.
+(*  
+  T_cases (induction T1) Case;
+  intros; subst; simpl; eauto; try solve by inversion...
+  inv H1... split... inv H... admit. admit.
+*)
+  intros.
+  generalize H1; intro G.
+  apply sub_inversion_prod in G...
+  inv G. inv H2. inv H3. inv H4.
+  inv H2...
+(*  
+  intros.
+  remember (TProd U1 U2) as rem.
+  generalize dependent T1.
+  generalize dependent T2.
+  generalize dependent U1.
+  generalize dependent U2.
+  induction H0; intros; subst; simpl; eauto; try solve by inversion.
+  inv Heqrem...
+  
+  intros.
+  remember (TProd T1 T2) as rem1.
+  remember (TProd U1 U2) as rem2.  
+  generalize dependent T1.
+  generalize dependent T2.
+  generalize dependent U1.
+  generalize dependent U2.  
+  subtype_cases (induction H1) Case;
+    intros; subst; simpl; eauto; try solve by inversion...
+  inv Heqrem1... inv H...
+*)
+Qed.
+  
 Theorem preservation : forall t t' T,
      empty |- t \in T  ->
      t ==> t'  ->
@@ -1474,8 +3147,29 @@ Proof with eauto.
     SCase "ST_AppAbs".
       destruct (abs_arrow _ _ _ _ _ HT1) as [HA1 HA2].
       apply substitution_preserves_typing with T...
+      econstructor. apply has_subtype__wf in HA1... inv HA1... apply HT2. auto.
+  Case "T_Fst".
+    inv HT... apply typing_inversion_pair in H2... inv H2. inv H4. inv H2. inv H5.
+    assert(G : TProd x x0 <: TProd T1 T2) by eauto.
+    apply prod_order in G. inv G.
+    econstructor... apply has_subtype__wf in H5. inv H5...
+    econstructor; eauto using has_type__wf. apply has_subtype__wf in G. inv G...
+  Case "T_Snd".
+    inv HT... apply typing_inversion_pair in H2... inv H2. inv H4. inv H2. inv H5.
+    assert(G : TProd x x0 <: TProd T1 T2) by eauto.
+    apply prod_order in G. inv G.
+    econstructor... apply has_subtype__wf in H7. inv H7...
+    econstructor; eauto using has_type__wf. apply has_subtype__wf in G. inv G...
+  Case "T_Proj".
+    apply lookup_field_in_value with (T:=Tr) (i:=i) (Ti:= Ti) in H2...
+    inv H2. inv H0. inv H1. inv H2.
+    rewrite H4 in H0. inv H0. eapply T_Sub...
+    apply has_subtype__wf in H3. inv H3...
+  Case "T_RCons".
+    constructor...
+    eapply step_preserves_record_tm...
 Qed.
-
+    
 (** ** Records, via Products and Top *)
 
 (** This formalization of the STLC with subtyping has omitted record
@@ -1549,6 +3243,7 @@ Qed.
 
 []
 *) 
+(* Gonna skip this *)
 
 (* ###################################################################### *)
 (** * Exercise: Adding Products *)
